spot/GC.SPOT.HeapExpansion.fst
@@ -193,6 +193,55 @@ let spot_chunked_all_minor_edges_preserved_by_expansion
   = CG.chunked_all_minor_edges_preserved_by_expansion
       ms mh fresh fp objs idx
 
+let spot_build_chunked_combined_graph_from_major_objects
+  (ms: minor_state) (mh: MH.major_heap) (major_objs: Seq.seq obj_addr)
+  : GTot CG.combined_graph
+  = CG.build_chunked_combined_graph_from_major_objects ms mh major_objs
+
+let spot_build_chunked_combined_graph
+  (ms: minor_state) (mh: MH.major_heap)
+  : GTot CG.combined_graph
+  = CG.build_chunked_combined_graph ms mh
+
+let spot_chunked_combined_graph_old_view_preserved_by_expansion
+  (ms: minor_state) (mh: MH.major_heap) (fresh: MH.heap_chunk) (fp: U64.t)
+  (major_objs: Seq.seq obj_addr)
+  : Lemma
+      (requires MH.chunk_disjoint_from_all fresh mh /\
+                CG.chunked_all_minor_expansion_safe
+                  ms fresh (minor_objects ms) 0 /\
+                CG.chunked_all_major_object_expansion_safe
+                  mh fresh major_objs 0)
+      (ensures (
+        let mh' = (SpecMajorAlloc.expand_major_heap mh fresh fp).major_out in
+        let g' =
+          spot_build_chunked_combined_graph_from_major_objects
+            ms mh' major_objs in
+        let g =
+          spot_build_chunked_combined_graph_from_major_objects
+            ms mh major_objs in
+        g'.cg_vertices == g.cg_vertices /\ g'.cg_edges == g.cg_edges))
+  = CG.chunked_combined_graph_old_view_preserved_by_expansion
+      ms mh fresh fp major_objs
+
+let spot_chunked_build_combined_graph_old_view_preserved_by_expansion
+  (ms: minor_state) (mh: MH.major_heap) (fresh: MH.heap_chunk) (fp: U64.t)
+  : Lemma
+      (requires MH.chunk_disjoint_from_all fresh mh /\
+                CG.chunked_all_minor_expansion_safe
+                  ms fresh (minor_objects ms) 0 /\
+                CG.chunked_all_major_object_expansion_safe
+                  mh fresh (MH.major_objects mh) 0)
+      (ensures (
+        let mh' = (SpecMajorAlloc.expand_major_heap mh fresh fp).major_out in
+        let g' =
+          spot_build_chunked_combined_graph_from_major_objects
+            ms mh' (MH.major_objects mh) in
+        let g = spot_build_chunked_combined_graph ms mh in
+        g'.cg_vertices == g.cg_vertices /\ g'.cg_edges == g.cg_edges))
+  = CG.chunked_build_combined_graph_old_view_preserved_by_expansion
+      ms mh fresh fp
+
 let spot_chunked_header_of_object_preserved_by_expansion
   (mh: MH.major_heap) (fresh: MH.heap_chunk) (fp: U64.t) (obj: obj_addr)
   : Lemma
